code/experimental/curve25519/Hacl.Impl.Curve25519.Generic.fst
@@ -45,6 +45,13 @@ let fget_x (#s:field_spec) (h:mem) (p:point s) = feval h (gsub p 0ul (nlimb s))
 let fget_z (#s:field_spec) (h:mem) (p:point s) = feval h (gsub p (nlimb s) (nlimb s))
 let fget_xz (#s:field_spec) (h:mem) (p:point s) = fget_x h p, fget_z h p
 
+val state_inv_t:#s:field_spec -> h:mem -> f:felem s -> Type0
+let state_inv_t #s h f =
+  match s with
+  | M26 -> True
+  | M51 -> F51.mul_inv_t h f
+  | M64 -> True
+
 inline_for_extraction
 val scalar_bit:
     s:scalar
@@ -245,25 +252,40 @@ let point_add_and_double #s q nq nq_p1 tmp1 tmp2 =
 
 inline_for_extraction
 val point_double_:
-    #s:field_spec
-  -> nq: point s
+    #s:field_spec{s == M51 \/ s == M64}
+  -> nq:point s
   -> tmp1:lbuffer (limb s) (4ul *. nlimb s)
   -> tmp2:felem_wide2 s
   -> Stack unit
-    (requires fun h0 -> live h0 nq /\ live h0 tmp1 /\ live h0 tmp2)
+    (requires fun h0 ->
+      live h0 nq /\ live h0 tmp1 /\ live h0 tmp2 /\
+      disjoint nq tmp1 /\ disjoint nq tmp2 /\ disjoint tmp1 tmp2 /\
+      state_inv_t h0 (get_x nq) /\
+      state_inv_t h0 (get_z nq))
     (ensures  fun h0 _ h1 ->
       modifies (loc nq |+| loc tmp1 |+| loc tmp2) h0 h1 /\
+      state_inv_t h0 (get_x nq) /\
+      state_inv_t h0 (get_z nq) /\
       fget_xz h1 nq == S.double (fget_xz h0 nq))
 let point_double_ #s nq tmp1 tmp2 =
   let x2 = sub nq 0ul (nlimb s) in
   let z2 = sub nq (nlimb s) (nlimb s) in
+
   let a : felem s = sub tmp1 0ul (nlimb s) in
   let b : felem s = sub tmp1 (nlimb s) (nlimb s) in
   let d : felem s = sub tmp1 (2ul *. nlimb s) (nlimb s) in
   let c : felem s = sub tmp1 (3ul *. nlimb s) (nlimb s) in
+
   let ab : felem2 s = sub tmp1 0ul (2ul *. nlimb s) in
   let dc : felem2 s = sub tmp1 (2ul *. nlimb s) (2ul *. nlimb s) in
-  admit();
+  let h0 = ST.get () in
+  assert (gsub nq 0ul (nlimb s) == x2);
+  assert (gsub nq (nlimb s) (nlimb s) == z2);
+  assert (gsub ab 0ul (nlimb s) == a);
+  assert (gsub ab (nlimb s) (nlimb s) == b);
+  assert (gsub dc 0ul (nlimb s) == d);
+  assert (gsub dc (nlimb s) (nlimb s) == c);
+
   fadd a x2 z2; // a = x2 + z2
   fsub b x2 z2; // b = x2 - z2
 
@@ -271,7 +293,6 @@ let point_double_ #s nq tmp1 tmp2 =
   //fsqr d a;     // d = aa = a^2
   //fsqr c b;     // c = bb = b^2
   fsqr2 dc ab tmp2;     // d|c = aa | bb
-
   copy_felem a c;                           // a = bb
   fsub c d c;   // c = e = aa - bb
   fmul1 b c (u64 121665); // b = e * 121665
@@ -284,7 +305,7 @@ let point_double_ #s nq tmp1 tmp2 =
 
 (* WRAPPER to Prevent Inlining *)
 [@CInline]
-let point_double_26 (nq:point26) tmp1 tmp2 = point_double_ #M26 nq  tmp1 tmp2
+let point_double_26 (nq:point26) tmp1 tmp2 = admit(); point_double_ #M26 nq  tmp1 tmp2
 [@CInline]
 let point_double_51 (nq:point51) tmp1 tmp2 = point_double_ #M51 nq tmp1 tmp2
 [@CInline]
@@ -297,9 +318,15 @@ val point_double:
   -> tmp1:lbuffer (limb s) (4ul *. nlimb s)
   -> tmp2:felem_wide2 s
   -> Stack unit
-    (requires fun h0 -> live h0 nq /\ live h0 tmp1 /\ live h0 tmp2)
-    (ensures fun h0 _ h1 ->
+    (requires fun h0 ->
+      live h0 nq /\ live h0 tmp1 /\ live h0 tmp2 /\
+      disjoint nq tmp1 /\ disjoint nq tmp2 /\ disjoint tmp1 tmp2 /\
+      state_inv_t h0 (get_x nq) /\
+      state_inv_t h0 (get_z nq))
+    (ensures  fun h0 _ h1 ->
       modifies (loc nq |+| loc tmp1 |+| loc tmp2) h0 h1 /\
+      state_inv_t h0 (get_x nq) /\
+      state_inv_t h0 (get_z nq) /\
       fget_xz h1 nq == S.double (fget_xz h0 nq))
 let point_double #s nq tmp1 tmp2 =
   match s with
